dynamic auction activity rule theorems

isabelle/Auction/Sandbox/Trust.thy
@@ -19,7 +19,7 @@ Predicate
 "~~/src/HOL/Library/Code_Numeral"
 "~~/src/HOL/Library/Code_Char"
 "~~/src/HOL/UNITY/ListOrder"
-"~~/src/HOL/Library/Formal_Power_Series"
+(*"~~/src/HOL/Library/Formal_Power_Series"*)
 begin
 
 abbreviation "currentBidder l == (size l - (2::nat)) mod (l!0)" (* the first bidder has label 0 *)
@@ -159,31 +159,162 @@ abbreviation "pairWise Op l m == [Op (l!i) (m!i). i <- [0..<min (size l) (size m
 lemma lm01: assumes "n\<in>{0..<min (size l) (size m)}" shows "(pairWise Op l m)!n = Op (l!n) (m!n)"
 using assms by auto
 abbreviation "deltaBids (*step*) l == (* step # *) (pairWise (op -) (tl l) l)"
-value "filterpositions2 (%x. x>3) [1::nat,2]"
+
 lemma lm02: "min (size (tl l)) (size l)=size l - (1::nat)" by simp
-lemma lm03: assumes "n\<in>{0..<size (l::int list)-(1::nat)}" shows "(deltaBids l)!n=(l!(Suc n)) - ((l!n)::int)" using 
-assms lm02 length_tl nth_tl atLeastLessThan_iff diff_zero monoid_add_class.add.left_neutral 
-nth_map_upt by (metis (erased, lifting))
+
+
+lemma lm03: assumes "n\<in>{0..<(size l)-(1)}" (* why the brackets around 1??? *) shows 
+"(deltaBids l)!n = (l!(Suc n)) - (l!n)" using assms lm02 length_tl nth_tl atLeastLessThan_iff 
+diff_zero monoid_add_class.add.left_neutral nth_map_upt by (metis (erased, lifting))
+
+lemma lm03b: fixes l::"int list" (* remove *) assumes "n\<in>{0..<(size l)-(1)}" (* why the brackets around 1??? *) shows 
+"(deltaBids l)!n = (l!(Suc n)) - (l!n)" using assms lm02 length_tl nth_tl atLeastLessThan_iff 
+diff_zero monoid_add_class.add.left_neutral nth_map_upt by (metis (erased, lifting))
+
+lemma fixes l::"'a::ab_group_add list" shows 
+"(\<Sum>i = 0..<size l-(1::nat). nth l i) = listsum l" using assms sorry
+
+lemma "listsum (map (nth l) [0..<size l]) = listsum l" by (metis map_nth)
+value "deltaBids [0::int, 2, 78]"
+lemma "setsum (nth l) {0..<size l} = listsum l" using assms by (metis listsum_setsum_nth)
+
+lemma lm10: "setsum (nth (deltaBids l)) {0..<size l-(1)} = setsum (%i. (l!(Suc i) - l!i)) {0..<size l-(1)}"
+using assms lm03 Trust.lm02 atLeastLessThan_iff diff_zero length_upt nth_map set_upt setsum.cong
+by smt2
+
+lemma lm10b: fixes l::"int list" (*remove*)
+assumes "m\<le>size l - (1)" shows "setsum (nth (deltaBids l)) {0..<m} = setsum (%i. (l!(Suc i) - l!i)) {0..<m}"
+using assms lm03b unfolding setsum.cong by auto
+
+lemma lm04: fixes l::"'a::ab_group_add list" shows 
+"(\<Sum>i = 0..<size l. nth l (Suc i) - nth l i) = nth l (size l) - nth l 0"
+using setsum_Suc_diff 
+proof -
+  have f1: "\<forall>x\<^sub>9 x\<^sub>1\<^sub>4. Suc x\<^sub>9 \<le> x\<^sub>1\<^sub>4 \<longrightarrow> (\<exists>x\<^sub>1\<^sub>5. x\<^sub>1\<^sub>4 = Suc x\<^sub>1\<^sub>5)" using Suc_le_D by blast
+  obtain esk4\<^sub>2 :: "nat \<Rightarrow> nat \<Rightarrow> nat" where f2: "\<And>x\<^sub>1. x\<^sub>1 = 0 \<or> Suc 0 \<le> x\<^sub>1" by (metis (no_types) diff_is_0_eq' diff_zero not_less_eq_eq)
+  have "\<And>x\<^sub>1 x\<^sub>2. (\<Sum>R = 0..<Suc x\<^sub>2. x\<^sub>1 (Suc R) - (x\<^sub>1 R\<Colon>'a)) = x\<^sub>1 (Suc x\<^sub>2) - x\<^sub>1 0" by (simp add: atLeastLessThanSuc_atLeastAtMost setsum_Suc_diff)
+  then obtain esk4\<^sub>2 :: "nat \<Rightarrow> nat \<Rightarrow> nat" where "\<And>x\<^sub>1 x\<^sub>2. (\<Sum>R = 0..<x\<^sub>2. x\<^sub>1 (Suc R) - (x\<^sub>1 R\<Colon>'a)) = x\<^sub>1 x\<^sub>2 - x\<^sub>1 0 \<or> x\<^sub>2 = 0" using f1 f2 by (metis (no_types))
+  thus "(\<Sum>i = 0..<length l. l ! Suc i - l ! i) = l ! length l - l ! 0" by fastforce
+qed
+
+lemma lm04a: fixes l::"'a::ab_group_add list" shows 
+"(\<Sum>i = 0..<size l-(1). nth l (Suc i) - nth l i) = nth l (size l-(1)) - nth l 0" 
+using One_nat_def Suc_diff_1 atLeastLessThanSuc_atLeastAtMost atLeastLessThan_empty diff_Suc_Suc diff_is_0_eq' 
+diff_self diff_zero length_0_conv length_tl length_upt lessI nat_less_le neq0_conv set_upt setsum.cong 
+setsum.empty setsum_Suc_diff by smt2
+
+lemma lm04c: fixes l::"'a::ab_group_add list" shows
+"(\<Sum>i = 0..<m. l ! (Suc i) - l!i) = l!m - l!0" using 
+atLeastLessThanSuc_atLeastAtMost atLeastLessThan_empty 
+diff_self order_refl setsum_Suc_diff not0_implies_Suc le0 
+by (metis(no_types))
+
+corollary lm04b: fixes l::"int list" shows 
+"(\<Sum>i = 0..<size l-(1). nth l (Suc i) - nth l i) = nth l (size l-(1)) - nth l 0"
+using lm04a by blast
+
+corollary lm12: fixes l::"'a::ab_group_add list" shows 
+"setsum (nth (deltaBids l)) {0..<size l-(1)} = l!(size l - (1)) - l!0" 
+using assms lm04a lm10 by (metis (no_types))
+
+corollary lm12b: fixes l::"int list" (* remove *) assumes "i<size l" shows 
+"setsum (nth (deltaBids l)) {0..<i} = l!i - l!0" 
+proof -
+  have "i \<le> length l - 1" using assms by linarith
+  thus "setsum (op ! (deltaBids l)) {0..<i} = l ! i - l ! 0" by (metis (no_types) lm04c lm10b)
+qed
+
+corollary lm12c: fixes l::"int list" (* remove *) assumes "i<size l" shows 
+"setsum (nth (deltaBids l)) {0..<i} = l!i - (hd l)" using assms lm12b 
+drop_0 hd_drop_conv_nth by (metis (full_types) less_nat_zero_code neq0_conv)
+
+lemma lm06: "[n. n\<leftarrow>[0..<N], Q n] = [n\<leftarrow>[0..<N]. Q n]" by (induct N) auto 
+corollary lm06b: "filterpositions2 P l = [n<-[0..<size l]. P (l!n)]" unfolding lm06 
+filterpositions2_def by blast
+lemma lm07: "sorted [n\<leftarrow>[0..<N]. Q n]" by (metis (full_types) map_ident sorted_filter sorted_upt)
+corollary lm07b: "sorted (filterpositions2 P l)" using lm07 lm06 unfolding filterpositions2_def by presburger
+
+corollary lm11: assumes "sorted l" "x \<ge> Max (set l)" shows "sorted (l@[x])" 
+using assms(1,2) sorted_append dual_order.trans by fastforce
+
+lemma lm08: assumes "m < Min A" "finite A" shows "m \<notin> A" using assms by (metis Min.boundedE equals0D not_less not_less_iff_gr_or_eq)
+
+lemma lm13: assumes "sorted l" "set l \<noteq> {}" shows "Min (set l)=hd l" using assms sorted.cases
+List.finite_set Min_in insert_iff le_neq_trans list.sel(1) lm08 set_simps(2)
+set_empty by (metis(no_types)) 
+(*
+proof -
+  have f1: "l \<noteq> []" using assms(2) by fastforce
+  have "\<And>v. \<forall>w. \<exists>uu uua. (sorted w \<longrightarrow> w = [] \<or> (uu\<Colon>'a) # uua = w) \<and> (sorted w \<and> v \<in> set uua \<longrightarrow> w = [] \<or> uu \<le> v)" by (metis (no_types) sorted.cases)
+  thus "Min (set l) = hd l" using f1 by (metis (no_types) List.finite_set Min_in assms(1) assms(2) insert_iff le_neq_trans list.sel(1) lm08 set_simps(2))
+qed
+*)
+
+lemma lm09: assumes "set [n\<leftarrow>[0..<N]. P n] \<noteq> {}" "m<Min (set [n\<leftarrow>[0..<N]. P n])" shows "\<not> (P m)" 
+using assms Min_in lm08 by fastforce
+
+corollary lm09c: assumes "set [(n::nat)\<leftarrow>[0..<N]. P n] \<noteq> {}" "m<hd [n<-[0..<N]. P n]" shows "\<not> (P m)"
+using assms lm07 lm09 lm13 by metis
+corollary lm09b: assumes "set (filterpositions2 P l) \<noteq> {}" "m<hd (filterpositions2 P l)" shows
+"\<not> (P (l!m))" using assms lm06b lm09c by metis
+
+lemma lm14: "filter P l = [x<-l. P x]" by blast
+lemma "[x<-l. P x] = map (nth l) [n<-[0..<size l]. P (nth l n)]" using nth_map sorry
+
+lemma lm15a: "(nth l)`(set ([n<-[0..<size l]. P (l!n)])) \<supseteq> {y\<in>set l. P y}"
+using imageE image_eqI  map_nth mem_Collect_eq  set_filter set_map subsetI by smt2
+lemma lm15: "(nth l)`(set ([n<-[0..<size l]. P (l!n)])) = (set l) \<inter> (P-`{True})" using lm15a by force
+
+lemma lm16: assumes "P y" "y\<in>set l" shows "y \<in> (nth l)`(set (filterpositions2 P l))" 
+using assms lm15 unfolding lm06b by force
+
+lemma lm17: assumes "m < hd (filterpositions2 (%x. x<step) (deltaBids (*step*) l)@[size l-(1)])"
+shows "\<not> ((deltaBids l)!m < step)" 
+proof -
+let ?l="filterpositions2 (%x. x<step) (deltaBids l)"
+have "?l=[] \<longrightarrow> (\<forall>x \<in> set (deltaBids l). \<not> (x<step))" 
+using lm16 by (smt2 empty_iff list.simps(8) set_empty set_map)
+moreover have "?l \<noteq> [] \<longrightarrow> ?thesis" using assms lm09b by (metis (mono_tags) empty_iff hd_append2 list.sel_set(1))
+ultimately show ?thesis using assms by fastforce
+qed
+lemma lm18: "set (filterpositions2 P l) \<subseteq> {0..<size l}" sorry
+corollary lm02b: "size (deltaBids l) = size l - 1" by (metis Trust.lm02 diff_zero length_map length_upt)
+corollary "hd (filterpositions2 (%x. x<step) (deltaBids (*step*) l)@[size l-(1)]) \<in> {0..<size l}" using lm18
+proof -
+let ?d="deltaBids l" let ?l="filterpositions2 (%x. x<step) ?d"
+{
+  assume 0: "?l \<noteq> []" then have "hd ?l \<in> {0..<size ?d}" using lm18 by (metis (erased, lifting) hd_in_set subsetCE)
+  then have ?thesis using lm02b 0 by fastforce
+}
+{ assume "?l=[]" then have ?thesis sorry }
+show ?thesis sorry
+qed
 abbreviation "firstInvalidBidIndex step l == 
-1 + hd (filterpositions2 (%x. x<step) (deltaBids (*step*) l)@[size l])"
-value "deltaBids [1::int, 5, 11]"
-
-lemma assumes "size l \<ge>2" "0\<le>size l - (2::int) + 1" shows "listsum (deltaBids l) = (\<Sum>i = 0..(size l - 2). (nth l)(Suc i) - (nth l) i)" 
-using assms sledgehammer
-
-lemma assumes "size l \<ge>2" shows "listsum (deltaBids l) = (l!(size l - (1::nat))) - (l!0)" 
-using assms setsum_natinterval_difff setsum_Suc_diff sorry
-
-lemma fixes f::"nat => real" shows "setsum (%x. f (x+1) - f x) {0..<Suc n}=f (Suc n) - f 0"
-using assms setsum_natinterval_difff setsum_Suc_diff sorry
+1 + hd (filterpositions2 (%x. x<step) (deltaBids (*step*) l)@[size l-(1)])"
+lemma "firstInvalidBidIndex step l
+\<in> {0..size l}" using lm18 sorry
+corollary lm17b: fixes l::"int list" assumes "m+1 < firstInvalidBidIndex step l"
+shows "step \<le> (deltaBids l)!m" using assms lm17 by fastforce
 
 
-lemma assumes "size (l::int list)\<ge>2" shows "listsum [l!(n+1)-(l!n). n<-[0..<size l - (1::nat)]]=l!(size l - (1::nat))-(l!0)"
-using assms setsum_natinterval_difff setsum_Suc_diff sorry
+lemma assumes "(n::nat)+1<firstInvalidBidIndex step l" shows "step \<le> (deltaBids l)!n"
+using assms
+ filterpositions2_def
+sorry
 
-lemma assumes "size l\<ge>2" shows "l!(size l-(1::nat))=listsum (deltaBids l) + ((l!0)::int)"
-using assms lm03 sorry
-
+lemma fixes l::"int list" assumes "(i::nat) < min (firstInvalidBidIndex (step::nat) l) (size l)"
+shows "l!i \<ge> hd l + i*step" using assms 
+proof -
+have "\<forall>x \<in> {0..<i}. step \<le> (deltaBids l)!x" using assms lm17b by auto
+then have "setsum (nth (deltaBids l)) {0..<i} \<ge> 
+setsum (%x. int_of_nat step) {0..<i}" using setsum_mono by (metis (erased, lifting) int_of_nat_def)
+moreover have "setsum (%x. int_of_nat step) {0..<i} = i*step" 
+using int_of_nat_def by (metis atLeast0LessThan card_lessThan of_nat_mult setsum_constant)
+ultimately have "setsum (nth (deltaBids l)) {0..<i} \<ge> i*step" by presburger
+moreover have "l!i = hd l + setsum (nth (deltaBids l)) {0..<i}" using assms lm12c by auto
+ultimately have "l!i \<ge> hd l + i*step" by presburger
+thus ?thesis by (metis of_nat_mult)
+qed
 abbreviation "amendedbidlist3 step l == update2 l {firstInvalidBidIndex step l..<size l} (%x. 
 l!(firstInvalidBidIndex step l - 1))"
 
@@ -202,7 +333,7 @@ lemma assumes "step \<ge>(1::nat)" "firstInvalidBidIndex step (l::nat list)=Suc 
 setsum_natinterval_difff setsum_Suc_diff sorry
 
 
-abbreviation "EX02 == [0::nat, 2, 4, 6, 8, 11, 12, 11]"
+abbreviation "EX02 == [0::nat, 2, 4, 6, 8, 11, 12, 15]"
 value "firstInvalidBidIndex 2 EX02"
 value "amendedbidlist3 2 EX02"
 
@@ -223,6 +354,15 @@ shows "EX M n. \<forall> l\<in> X. (\<forall>m. (m > n & m < size l) \<longright
 using assms sorry
 
 (* abbreviation "allowedBids bidSet bid == " activity rule*)
+
+(*
+lemma lm09: assumes "set l \<noteq> {}" "sorted l" "x \<ge> Max (set l)" "finite (set l)" shows "sorted (l@[x])" 
+using assms sorted_append sorted_single Max.bounded_iff ball_empty list.set(1) set_ConsD by (metis (mono_tags, lifting) )
+corollary lm09c: assumes "set l \<noteq> {}" "sorted l" "x \<ge> Sup (set l)" shows "sorted (l@[x])"
+using assms lm09 Max_Sup List.finite_set
+sorry
+using assms lm09 sorted_single append_Nil set_empty2 List.finite_set Max_Sup sorry
+*)
 
 end
 
